\documentclass{article}
\usepackage{ifthen}
\usepackage{epsfig}
\usepackage[utf8]{inputenc}
\usepackage{newunicodechar}
  \newunicodechar{⁻}{${}^{-}$}% Superscript minus
  \newunicodechar{²}{${}^{2}$}% Superscript two
  \newunicodechar{³}{${}^{3}$}% Superscript three

\pagestyle{empty}
\begin{document}
$ |x| $
\pagebreak

$ x \in [-1,1] $
\pagebreak

\[ \text{acos}(x) = \text{atan} \left( \frac{\sqrt{1-x^2}}{x} \right) \]
\pagebreak

\[ \text{acosh}(x) = \ln \left( x + \sqrt{x^2 - 1} \right) \]
\pagebreak

\[ \text{asin}(x) = \text{atan} \left( \frac{x}{\sqrt{1-x^2}} \right) \]
\pagebreak

\[ \text{asinh}(x) = \ln \left( x + \sqrt{x^2 + 1} \right) \]
\pagebreak

\[ \text{atan}(x) = \dfrac{x}{1 + \dfrac{x^2}{3 + \dfrac{4x^2}{5 + \dfrac{9x^2}{7 + \ddots}}}} \]
\pagebreak

\[ \text{atan2}(y,x) = \begin{cases} \text{atan}(y/x) & \text{ if } x > 0 \\ \text{atan}(y/x) + \pi & \text{ if } x < 0 \text{ and } y \geq 0 \\ \text{atan}(y/x) - \pi & \text{ if } x < 0 \text{ and } y < 0 \\ + \pi/2 & \text{ if } x = 0 \text{ and } y > 0 \\ - \pi/2 & \text{ if } x = 0 \text{ and } y < 0 \end{cases} \]
\pagebreak

\[ \text{atan2}(y,x) = \begin{cases} +0 & \text{ if } x = +0 \text{ and } y = +0 \\ -0 & \text{ if } x = +0 \text{ and } y = -0 \\ +\pi & \text{ if } x = -0 \text{ and } y = +0 \\ - \pi & \text{ if } x = -0 \text{ and } y = -0 \end{cases} \]
\pagebreak

\[ \text{atanh}(x) = \frac{1}{2} \ln \left( \frac{1+x}{1-x} \right) \]
\pagebreak

\[ \text{B}(\alpha,\beta) := \int_0^1 t^{\alpha - 1} (1-t)^{\beta - 1} dt = \frac{\Gamma(\alpha)\Gamma(\beta)}{\Gamma(\alpha + \beta)} \]
\pagebreak

$ \Gamma $
\pagebreak

\[ \binom{n}{k} = \frac{n!}{k!(n-k)!} \]
\pagebreak

\[ \cos(x) = \frac{1-\tan^2(x/2)}{1+\tan^2(x/2)} \]
\pagebreak

\[ \cosh(x) = \frac{\exp(x) + \exp(-x)}{2} \]
\pagebreak

\[ \text{erf}(x) = \frac{2}{\sqrt{\pi}} \int_0^x \exp( - t^2) dt \]
\pagebreak

\[ \text{erf}(x) = \frac{2x}{\sqrt{\pi}} \exp(-x^2) \dfrac{1}{1 - 2x^2 + \dfrac{4x^2}{3 - 2x^2 + \dfrac{8x^2}{5 - 2x^2 + \dfrac{12x^2}{7 - 2x^2 + \ddots}}}} \]
\pagebreak

$ x $
\pagebreak

\[ f(x) := \text{erf}(x) - p \]
\pagebreak

\[ x_{n+1} = x_n - \frac{f(x_n)/f'(x_n)}{1 - 0.5 \frac{f(x_n)}{f'(x_n)} \frac{f''(x_n)}{f'(x_n)} } \]
\pagebreak

\[ \frac{\partial}{\partial x} \text{erf}(x) = \exp(-x^2), \ \ \frac{\partial^2}{\partial x^2} \text{erf}(x) = -2x\exp(-x^2) \]
\pagebreak

$ \exp(x) $
\pagebreak

\[ \exp(x) = \dfrac{1}{1-\dfrac{x}{1+x-\dfrac{\frac{1}{2}x}{1 + \frac{1}{2}x - \dfrac{\frac{1}{3}x}{1 + \frac{1}{3}x - \ddots}}}} \]
\pagebreak

$ x = n + r $
\pagebreak

$ n $
\pagebreak

$ r \in [-0.5,0.5] $
\pagebreak

$ \exp(x) - 1 $
\pagebreak

\[ \exp(x) = \sum_{k=0}^\infty \dfrac{x^k}{k!} \]
\pagebreak

$ x! $
\pagebreak

$ x / y $
\pagebreak

\[ \text{fmod}(x,y) = x - \text{trunc}(x/y) \times y \]
\pagebreak

\[ \frac{\text{B}(z;\alpha,\beta)}{\text{B}(\alpha,\beta)} = \frac{1}{\text{B}(\alpha,\beta)}\int_0^z t^{a-1} (1-t)^{\beta-1} dt \]
\pagebreak

\[ \frac{\text{B}(z;\alpha,\beta)}{\text{B}(\alpha,\beta)} = \frac{z^{\alpha} (1-t)^{\beta}}{\alpha \text{B}(\alpha,\beta)} \dfrac{a_1}{1 + \dfrac{a_2}{1 + \dfrac{a_3}{1 + \dfrac{a_4}{1 + \ddots}}}} \]
\pagebreak

$ a_1 = 1 $
\pagebreak

\[ a_{2m+2} = - \frac{(\alpha + m)(\alpha + \beta + m)}{(\alpha + 2m)(\alpha + 2m + 1)}, \ m \geq 0 \]
\pagebreak

\[ a_{2m+1} = \frac{m(\beta - m)}{(\alpha + 2m - 1)(\alpha + 2m)}, \ m \geq 1 \]
\pagebreak

$ f_j $
\pagebreak

$ j $
\pagebreak

\[ c_j = 1 + a_j / c_{j-1}, \ \ d_j = 1 / (1 + a_j d_{j-1}) \]
\pagebreak

\[ f_j = c_j d_j f_{j-1} \]
\pagebreak

\[ f(x) := \frac{\text{B}(x;\alpha,\beta)}{\text{B}(\alpha,\beta)} - p \]
\pagebreak

\[ \frac{\partial}{\partial x} \left(\frac{\text{B}(x;\alpha,\beta)}{\text{B}(\alpha,\beta)}\right) = \frac{1}{\text{B}(\alpha,\beta)} x^{\alpha-1} (1-x)^{\beta-1} \]
\pagebreak

\[ \frac{\partial^2}{\partial x^2} \left(\frac{\text{B}(x;\alpha,\beta)}{\text{B}(\alpha,\beta)}\right) = \frac{1}{\text{B}(\alpha,\beta)} x^{\alpha-1} (1-x)^{\beta-1} \left( \frac{\alpha-1}{x} - \frac{\beta-1}{1 - x} \right) \]
\pagebreak

\[ \frac{\gamma(a,x)}{\Gamma(a)} = \frac{1}{\Gamma(a)} \int_0^x t^{a-1} \exp(-t) dt \]
\pagebreak

$ \Gamma(a,x) $
\pagebreak

\[ \Gamma(a,x) = \Gamma(a) - \dfrac{x^a\exp(-x)}{a - \dfrac{ax}{a + 1 + \dfrac{x}{a + 2 - \dfrac{(a+1)x}{a + 3 + \dfrac{2x}{a + 4 - \ddots}}}}} \]
\pagebreak

$ \gamma(a,x) $
\pagebreak

\[ \frac{\gamma(a,x)}{\Gamma(a)} + \frac{\Gamma(a,x)}{\Gamma(a)} = 1 \]
\pagebreak

$ a > 10 $
\pagebreak

\[ f(x) := \frac{\gamma(a,x)}{\Gamma(a)} - p \]
\pagebreak

\[ \frac{\partial}{\partial x} \left(\frac{\gamma(a,x)}{\Gamma(a)}\right) = \frac{1}{\Gamma(a)} x^{a-1} \exp(-x) \]
\pagebreak

\[ \frac{\partial^2}{\partial x^2} \left(\frac{\gamma(a,x)}{\Gamma(a)}\right) = \frac{1}{\Gamma(a)} x^{a-1} \exp(-x) \left( \frac{a-1}{x} - 1 \right) \]
\pagebreak

\[ \ln \text{B}(\alpha,\beta) := \ln \int_0^1 t^{\alpha - 1} (1-t)^{\beta - 1} dt = \ln \Gamma(\alpha) + \ln \Gamma(\beta) - \ln \Gamma(\alpha + \beta) \]
\pagebreak

\[ \text{lcm}(a,b) = \dfrac{| a b |}{\text{gcd}(a,b)} \]
\pagebreak

$ \text{gcd}(a,b) $
\pagebreak

$ a $
\pagebreak

$ b $
\pagebreak

\[ \ln \Gamma(x) = \ln \int_0^\infty y^{x-1} \exp(-y) dy \]
\pagebreak

\[ \Gamma(x+1) \approx (x+g+0.5)^{x+0.5} \exp(-x-g-0.5) \sqrt{2 \pi} \left[ c_0 + \frac{c_1}{x+1} + \frac{c_2}{x+2} + \cdots + \frac{c_n}{x+n} \right] \]
\pagebreak

$ g $
\pagebreak

$ (c_0, c_1, \ldots, c_n) $
\pagebreak

\[ \Gamma_p(a) = \pi^{(p-1)/2} \Gamma(a) \Gamma_{p-1}(a-0.5) \]
\pagebreak

$ \Gamma_1(a) = \Gamma(a) $
\pagebreak

$ \log_e(x) $
\pagebreak

\[ \log\left(\frac{1+x}{1-x}\right) = \dfrac{2x}{1-\dfrac{x^2}{3-\dfrac{4x^2}{5 - \dfrac{9x^3}{7 - \ddots}}}}, \ \ x \in [-1,1] \]
\pagebreak

$ x = a \times 10^c $
\pagebreak

$ c $
\pagebreak

$ \log_e(x+1) $
\pagebreak

\[ \log(x+1) = \sum_{k=1}^\infty \dfrac{(-1)^{k-1}x^k}{k}, \ \ |x| < 1 \]
\pagebreak

$ \log_2(x) $
\pagebreak

\[ \log_{2}(x) = \frac{\log_e(x)}{\log_e(2)} \]
\pagebreak

\[ \ln \frac{n!}{k!(n-k)!} = \ln \Gamma(n+1) - [ \ln \Gamma(k+1) + \ln \Gamma(n-k+1) ] \]
\pagebreak

$ \text{base}^{\text{exp\_term}} = e^{\text{exp\_term} \log(\text{base})} $
\pagebreak

$ y $
\pagebreak

\[ y = \begin{cases} 1 \ &\text{ if } x > 0 \\ 0 \ &\text{ if } x = 0 \\ -1 \ &\text{ if } x < 0 \end{cases} \]
\pagebreak

\[ \sin(x) = \frac{2\tan(x/2)}{1+\tan^2(x/2)} \]
\pagebreak

\[ \sinh(x) = \frac{\exp(x) - \exp(-x)}{2} \]
\pagebreak

$ \sqrt{x} $
\pagebreak

\[ \tan(x) = \dfrac{x}{1 - \dfrac{x^2}{3 - \dfrac{x^2}{5 - \ddots}}} \]
\pagebreak

$ \pi / 2 $
\pagebreak

\[ \tan(x) = - \frac{1}{x-\pi/2} - \sum_{k=1}^\infty \frac{(-1)^k 2^{2k} B_{2k}}{(2k)!} (x - \pi/2)^{2k - 1} \]
\pagebreak

$ B_n $
\pagebreak

\[ \tanh(x) = \dfrac{x}{1 + \dfrac{x^2}{3 + \dfrac{x^2}{5 + \dfrac{x^2}{7 + \ddots}}}} \]
\pagebreak

\[ \Gamma(x) = \int_0^\infty y^{x-1} \exp(-y) dy \]
\pagebreak

\end{document}
